Checkpoint

src/tls/Old.Handshake.fst
@@ -40,7 +40,6 @@ unfold val trace: s:string -> ST unit
   (ensures (fun h0 _ h1 -> h0 == h1))
 unfold let trace = if DebugFlags.debug_HS then print else (fun _ -> ())
 
-
 // TODO : implement resumption
 //val getCachedSession: cfg:config -> ch:ch -> ST (option session)
 //  (requires (fun h -> True))
@@ -755,29 +754,29 @@ let serverHello (m:Nego.mode) =
 
 type binders = Parsers.OfferedPsks_binders.offeredPsks_binders
 
-val  consistent_truncation: option Extensions.offeredPsks -> option binders -> bool
-let consistent_truncation x y =
-  match x, y with
-  | None, None -> true
-  | None, Some _ -> false
-  | Some _, None -> false
-  | Some psks, Some binders -> List.length psks.Extensions.identities = List.length binders
+val  consistent_truncation: option Extensions.offeredPsks -> bool
+let consistent_truncation x =
+  match x with
+  | None -> true
+  | Some psk -> List.length psk.Extensions.identities = List.length psk.Extensions.binders
 
 (* receive ClientHello, choose a protocol version and mode *)
-val server_ClientHello: hs -> HSM.clientHello -> option binders -> ST incoming
+val server_ClientHello: hs -> HSM.clientHello -> ST incoming
   (requires (fun h -> True))
   (ensures (fun h0 i h1 -> True))
-let server_ClientHello hs offer obinders =
-    trace ("Processing ClientHello"
-           ^ (if Some? obinders
-              then " with "
-                   ^ string_of_int (List.length (Some?.v obinders))
-                   ^ " binder(s)"
-              else ""));
 
-    // Check consistency across the truncated PSK extension (is is redundant?)
-    let opsk = Nego.find_clientPske offer in
-    if not (consistent_truncation opsk obinders)
+let server_ClientHello hs offer =
+  let open Parsers.OfferedPsks in
+  let binders = Nego.find_clientPske offer in
+
+    trace ("Processing ClientHello"
+           ^ (match binders with
+	     | None -> ""
+             | Some opsk -> " with "
+	       ^ string_of_int (List.length opsk.binders)
+               ^ " binder(s)"));
+
+    if not (consistent_truncation binders)
     then InError (fatalAlert Illegal_parameter, "unexpected number of binders")
     else
 
@@ -822,13 +821,13 @@ let server_ClientHello hs offer obinders =
         let digestSessionTicket =
           if Nego.sendticket_12 mode then
             // Save hashing the SH if we don't send a ticket
-            let _ = HandshakeLog.send hs.log (HSL.Msg (HSM.M_server_hello serverHello mode)) in
+            let _ = HandshakeLog.send hs.log (HSL.Msg (serverHello mode)) in
             let ticket =
 	      let open Parsers.NewSessionTicket12 in
 	      {lifetime_hint = 3600ul; ticket = tid; } in
             HandshakeLog.send_tag #ha hs.log (HSL.Msg12 (HSM.M12_new_session_ticket ticket))
           else
-            HandshakeLog.send_tag #ha hs.log (HSL.Msg (HSM.M_server_hello serverHello mode))
+            HandshakeLog.send_tag #ha hs.log (HSL.Msg (serverHello mode))
           in
         let digestServerFinished =
           let fink = KeySchedule.ks_12_finished_key hs.ks in
@@ -849,13 +848,13 @@ let server_ClientHello hs offer obinders =
         | Some i -> (
             trace ("accepted TLS 1.3 psk #"^string_of_int i);
             // we should statically know that the offer list is big enough, hence the binder list too.
-            let Some psks = opsk in
+            let Some psks = binders in
 	    let tlen = Extensions.offeredPsks_binders_size32 psks.Extensions.binders in
             let Some id = List.Tot.nth psks.Extensions.identities i in
-            let Some tag = List.Tot.nth (Some?.v obinders) i in
+            let Some tag = List.Tot.nth psks.Extensions.binders i in
             assume(PSK.registered_psk id.Extensions.identity);
             let server_share, Some binderKey = KeySchedule.ks_server_13_init hs.ks cr cs (Some id.Extensions.identity) g_gx in
-            if verify_binder hs binderKey tag (UInt32.v tlen)
+            if verify_binder hs binderKey tag tlen
             then Correct server_share
             else
               //( trace ("WARNING: binder verification failed, tlen="^string_of_int tlen); Correct server_share))
@@ -878,7 +877,7 @@ let server_ClientHello hs offer obinders =
         let ha = verifyDataHashAlg_of_ciphersuite mode.Nego.n_cipher_suite in
         // these hashes are not always used
         let digestClientHelloBinders = HandshakeLog.hash_tag #ha hs.log in
-        let digestServerHello = HandshakeLog.send_tag #ha hs.log (serverHello mode) in
+        let digestServerHello = HandshakeLog.send_tag #ha hs.log (HSL.Msg (serverHello mode)) in
         if pv = TLS_1p3
         then
           begin
@@ -904,29 +903,24 @@ let server_ClientHello hs offer obinders =
           server_ServerHelloDone hs // sending our whole flight hopefully in a single packet.
     )
 
+inline_for_extraction type cke_t = Parsers.Handshake12_m12_client_key_exchange.handshake12_m12_client_key_exchange
+
 (* receive ClientKeyExchange; CCS *)
-let server_ClientCCS1 hs cke (* clientCert *) digestCCS1 =
+let server_ClientCCS1 hs (cke:cke_t) (* clientCert *) digestCCS1 =
     // FIXME support optional client c and cv
     // let ems = n.n_extensions.ne_extended_ms in // ask Nego?
     trace "process Client CCS";
-    match cke.cke_kex_c with
-      | KEX_C_RSA _ | KEX_C_DH -> InError(fatalAlert Decode_error, perror __SOURCE_FILE__ __LINE__ "Expected DHE/ECDHE CKE")
-      | KEX_C_DHE gyb
-      | KEX_C_ECDHE gyb ->
-        begin
-          let mode = Nego.getMode hs.nego in  //TODO read back from mode.
-          // ADL: the type of gyb will change from bytes to g & share g; for now we parse here.
-          let Some (|g,  _|) = mode.Nego.n_server_share in
-          match CommonDH.parse g gyb with
-          | None -> InError(fatalAlert Decode_error, perror __SOURCE_FILE__ __LINE__ "Cannot parse client share in CKE")
-          | Some gy ->
-            let app_keys = KeySchedule.ks_server_12_cke_dh hs.ks (| g, gy |) digestCCS1 in
-            register hs app_keys;
-            Epochs.incr_reader hs.epochs;
-            // use the new reader; will use the new writer only after sending CCS
-            hs.state := S_Wait_Finished1 digestCCS1; // keep digest to verify the Client Finished
-            InAck true false  // Server 1.2 ATK
-        end
+    let mode = Nego.getMode hs.nego in
+    let Some (|g,  _|) = mode.Nego.n_server_share in
+    match CommonDH.parse g cke with
+    | None -> InError(fatalAlert Decode_error, perror __SOURCE_FILE__ __LINE__ "Cannot parse client share in CKE")
+    | Some gy ->
+      let app_keys = KeySchedule.ks_server_12_cke_dh hs.ks (| g, gy |) digestCCS1 in
+      register hs app_keys;
+      Epochs.incr_reader hs.epochs;
+      // use the new reader; will use the new writer only after sending CCS
+      hs.state := S_Wait_Finished1 digestCCS1; // keep digest to verify the Client Finished
+      InAck true false  // Server 1.2 ATK
 
 // Resumption client finished
 let server_ClientFinished2 hs cvd digestSF digestCF =
@@ -963,14 +957,14 @@ let server_ClientFinished hs cvd digestCCS digestClientFinished =
         if Nego.sendticket_12 mode then
           let (msId, ms) = KeySchedule.ks_12_ms hs.ks in
           let ticket = Ticket.Ticket12 pv cs (Nego.emsFlag mode) msId ms in
-          let ticket = {
-            sticket_lifetime = FStar.UInt32.(uint_to_t 3600);
-            sticket_ticket = Ticket.create_ticket false ticket;
-          } in
-          HandshakeLog.send_tag #ha hs.log (NewSessionTicket ticket)
+          let ticket = Parsers.NewSessionTicket12.({
+            lifetime_hint = 3600ul;
+            ticket = Ticket.create_ticket false ticket;
+          }) in
+          HandshakeLog.send_tag #ha hs.log (HSL.Msg12 (HSM.M12_new_session_ticket ticket))
         else digestClientFinished in
       let svd = TLSPRF.finished12 ha fink Server digestTicket in
-      let unused_digest = HandshakeLog.send_CCS_tag #ha hs.log (Finished ({fin_vd = svd})) true in
+      let unused_digest = HandshakeLog.send_CCS_tag #ha hs.log (HSL.Msg12 (HSM.M12_finished svd)) true in
       hs.state := S_Complete;
       InAck false false // Server 1.2 ATK; will switch write key and signal completion after sending
     else
@@ -997,22 +991,25 @@ let server_ServerFinished_13 hs i =
     let digestFinished =
       match kex with
       | Kex_ECDHE -> // [Certificate; CertificateVerify]
-        HandshakeLog.send hs.log (EncryptedExtensions eexts);
+        HandshakeLog.send hs.log (HSL.Msg13 (HSM.M13_encrypted_extensions eexts));
         let Some (chain, sa) = mode.Nego.n_server_cert in
-        let digestSig = HandshakeLog.send_tag #halg hs.log (Certificate13 ({crt_request_context = empty_bytes; crt_chain13 = chain})) in
+	let c = Parsers.Certificate13.({
+	  certificate_request_context = empty_bytes;
+	  certificate_list = chain}) in
+        let digestSig = HandshakeLog.send_tag #halg hs.log (HSL.Msg13 (HSM.M13_certificate c)) in
         let tbs = Nego.to_be_signed pv Server None digestSig in
         (match Nego.sign hs.nego tbs with
         | Error z -> Error z
-        | Correct signature -> Correct (HandshakeLog.send_tag #halg hs.log (CertificateVerify (signature))))
+        | Correct signature -> Correct (HandshakeLog.send_tag #halg hs.log (HSL.Msg13 (HSM.M13_certificate_verify signature))))
       | _ -> // PSK
-        Correct (HandshakeLog.send_tag #halg hs.log (EncryptedExtensions eexts))
+        Correct (HandshakeLog.send_tag #halg hs.log (HSL.Msg13 (HSM.M13_encrypted_extensions eexts)))
       in
 
     match digestFinished with
     | Correct digestFinished ->
       let (| sfinId, sfin_key |) = KeySchedule.ks_server_13_server_finished hs.ks in
       let svd = HMAC_UFCMA.mac sfin_key digestFinished in
-      let digestServerFinished = HandshakeLog.send_tag #halg hs.log (Finished ({fin_vd = svd})) in
+      let digestServerFinished = HandshakeLog.send_tag #halg hs.log (HSL.Msg13 (HSM.M13_finished svd)) in
       // we need to call KeyScheduke twice, to pass this digest
       let app_keys, exporter_master_secret = KeySchedule.ks_server_13_sf hs.ks digestServerFinished in
       export hs exporter_master_secret;
@@ -1055,20 +1052,22 @@ let server_Ticket hs (app_data:bytes) =
     | Some max_ed -> [NSTE_early_data max_ed]
     | None -> [] in
   let tnonce, _ = split_ tb 12 in
-  HandshakeLog.send hs.log (NewSessionTicket13 ({
-    ticket13_lifetime = FStar.UInt32.(uint_to_t 3600);
-    ticket13_age_add = age_add;
-    ticket13_nonce = tnonce;
-    ticket13_ticket = tb;
-    ticket13_extensions = ticket_ext;
-  }))
+  HandshakeLog.send hs.log (HSL.Msg13 (HSM.M13_new_session_ticket
+  Parsers.NewSessionTicket13.({
+    ticket_lifetime = 3600ul;
+    ticket_age_add = age_add;
+    ticket_nonce = tnonce;
+    ticket = tb;
+    extensions = ticket_ext;
+  })))
 
 (* receive ClientFinish 1.3 *)
 val server_ClientFinished_13: hs ->
   cvd:bytes ->
   Hashing.anyTag -> // Digest either up to ServerFinished or up to CertificateVerify with client certg
   Hashing.anyTag -> // Digest up to ClientFinished
-  option (HandshakeMessages.crt13 * HandshakeMessages.cv * Hashing.anyTag) -> St incoming
+  option (HSM.certificate13 * HSM.certificateVerify13 * Hashing.anyTag) ->
+  St incoming
 
 let server_ClientFinished_13 hs f digestBeforeClientFinished digestClientFinished clientAuth =
    trace "Process Client Finished";
@@ -1142,158 +1141,154 @@ let invalidateSession hs = ()
 
 let next_fragment_bounded (hs:hs) i (max:nat) =
     trace "next_fragment";
-    let outgoing = HandshakeLog.write_at_most hs.log i max in
+    let outgoing = HSL.write_at_most hs.log i max in
     match outgoing, !hs.state with
     // when the output buffer is empty, we send extra messages in two cases
     // we prepare the initial ClientHello; or
     // after sending ServerHello in plaintext, we continue with encrypted traffic
     // otherwise, we just returns buffered messages and signals
-    | Outgoing None None false, C_Idle ->
+    | HSL.Outgoing None None false, C_Idle ->
       (match client_ClientHello hs i with
       | Error z -> Error z
-      | Correct () -> Correct(HandshakeLog.write_at_most hs.log i max))
-    | Outgoing None None false, S_Sent_ServerHello ->
+      | Correct () -> Correct(HSL.write_at_most hs.log i max))
+    | HSL.Outgoing None None false, S_Sent_ServerHello ->
       (match server_ServerFinished_13 hs i with
       | Error z -> Error z
-      | Correct () -> Correct(HandshakeLog.write_at_most hs.log i max))
-    | Outgoing None None false, C_Sent_EOED d ocr cfk ->
+      | Correct () -> Correct(HSL.write_at_most hs.log i max))
+    | HSL.Outgoing None None false, C_Sent_EOED d ocr cfk ->
       client_ClientFinished_13 hs d ocr cfk;
-      Correct(HandshakeLog.write_at_most hs.log i max)
+      Correct(HSL.write_at_most hs.log i max)
     | _ -> Correct outgoing // nothing to do
 
 let next_fragment (hs:hs) i =
   next_fragment_bounded hs i max_TLSPlaintext_fragment_length
 
 let to_be_written (hs:hs) =
-  HandshakeLog.to_be_written hs.log
+  HSL.to_be_written hs.log
 
 (* ----------------------- Incoming ----------------------- *)
 
 let rec recv_fragment (hs:hs) #i rg f =
-    let  recv_again r =
-      match r with
-      | InAck false false -> recv_fragment hs #i (0,0) empty_bytes // only case where the next incoming flight may already have been buffered.
-      | r -> r  in
-    trace "recv_fragment";
-    let h0 = HST.get() in
-    let flight = HandshakeLog.receive hs.log f in
-    match flight with
-    | Error z -> InError z
-    | Correct None -> InAck false false // nothing happened
-    | Correct (Some (ms,ts)) ->
-      match !hs.state, ms, ts with
-      | C_Idle, _, _ -> InError (fatalAlert Unexpected_message, "Client hasn't sent hello yet")
+  let open HandshakeLog in
+  let open HandshakeMessages in
+  let recv_again r =
+    match r with
+    // only case where the next incoming flight may already have been buffered.
+    | InAck false false -> recv_fragment hs #i (0,0) empty_bytes
+    | r -> r  in
+  trace "recv_fragment";
+  let h0 = HST.get() in
+  let flight = receive hs.log f in
+  match flight with
+  | Error z -> InError z
+  | Correct None -> InAck false false // nothing happened
+  | Correct (Some (ms,ts)) ->
+    match !hs.state, ms, ts with
+    | C_Idle, _, _ -> InError (fatalAlert Unexpected_message, "Client hasn't sent hello yet")
+    | C_Wait_ServerHello, [Msg (M_server_hello sh)], [] ->
+      recv_again (client_ServerHello hs sh)
+//      | C_Wait_ServerHello, [HelloRetryRequest hrr], [] ->
+//        client_HelloRetryRequest hs hrr
+//  | C_Wait_ServerHello, Some ([ServerHello sh], [digest]) -> client_ServerHello hs sh digest
 
-      | C_Wait_ServerHello, [HelloRetryRequest hrr], [] ->
-        client_HelloRetryRequest hs hrr
+    | C_Wait_ServerHelloDone, [Msg12 (M12_certificate c); Msg12 (M12_server_key_exchange ske); Msg12 (M12_server_hello_done ())], [] ->
+      client_ServerHelloDone hs c ske None
 
-      | C_Wait_ServerHello, [ServerHello sh], [] ->
-        recv_again (client_ServerHello hs sh)
+    | C_Wait_ServerHelloDone, [Msg12 (M12_certificate c); Msg12 (M12_server_key_exchange ske); Msg12 (M12_certificate_request cr); Msg12 (M12_server_hello_done ())], [] ->
+      client_ServerHelloDone hs c ske (Some cr)
 
-    //| C_Wait_ServerHello, Some ([ServerHello sh], [digest]) -> client_ServerHello hs sh digest
-      | C_Wait_ServerHelloDone, [Certificate c; ServerKeyExchange ske; ServerHelloDone], [] ->
-        client_ServerHelloDone hs c ske None
+    | C_Wait_Finished1, [Msg13 (M13_encrypted_extensions ee); Msg13 (M13_certificate c); Msg13 (M13_certificate_verify cv); Msg13 (M13_finished f)],
+      [_; digestCert; digestCertVerify; digestServerFinished] ->
+      client_ServerFinished_13 hs ee None (Some c) (Some cv) f
+                               (Some digestCert) digestCertVerify digestServerFinished
 
-      | C_Wait_ServerHelloDone, [Certificate c; ServerKeyExchange ske; CertificateRequest cr; ServerHelloDone], [] ->
-        client_ServerHelloDone hs c ske (Some cr)
+    | C_Wait_Finished1, [Msg13 (M13_encrypted_extensions ee); Msg13 (M13_certificate_request cr); Msg13 (M13_certificate c); Msg13 (M13_certificate_verify cv); Msg13 (M13_finished f)],
+      [_; digestCert; digestCertVerify; digestServerFinished] ->
+      client_ServerFinished_13 hs ee (Some cr) (Some c) (Some cv) f
+                               (Some digestCert) digestCertVerify digestServerFinished
 
-      | C_Wait_Finished1, [EncryptedExtensions ee; Certificate13 c; CertificateVerify cv; Finished f],
-                          [_; digestCert; digestCertVerify; digestServerFinished] ->
-        client_ServerFinished_13 hs ee None (Some c) (Some cv) f.fin_vd
-                                 (Some digestCert) digestCertVerify digestServerFinished
+    | C_Wait_Finished1, [Msg13 (M13_encrypted_extensions ee); Msg13 (M13_finished f)],
+                        [digestEE; digestServerFinished] ->
+      client_ServerFinished_13 hs ee None None None f None digestEE digestServerFinished
 
-      | C_Wait_Finished1, [EncryptedExtensions ee; CertificateRequest13 cr; Certificate13 c; CertificateVerify cv; Finished f],
-                          [_; digestCert; digestCertVerify; digestServerFinished] ->
-        client_ServerFinished_13 hs ee (Some cr) (Some c) (Some cv) f.fin_vd
-                                 (Some digestCert) digestCertVerify digestServerFinished
+    | C_Wait_R_Finished1 digestNewSessionTicket, [Msg12 (M12_finished f)], [digestServerFinished] ->
+      client_R_ServerFinished hs f digestNewSessionTicket digestServerFinished
 
-      | C_Wait_Finished1, [EncryptedExtensions ee; Finished f],
-                          [digestEE; digestServerFinished] ->
-       client_ServerFinished_13 hs ee None None None f.fin_vd None digestEE digestServerFinished
+    | C_Wait_Finished2 digestClientFinished, [Msg12 (M12_finished f)], [digestServerFinished] ->
+      client_ServerFinished hs f digestClientFinished
 
-      | C_Wait_R_Finished1 digestNewSessionTicket, [Finished f], [digestServerFinished] ->
-        client_R_ServerFinished hs f digestNewSessionTicket digestServerFinished
+    | S_Idle, [Msg (M_client_hello ch)], []  -> server_ClientHello hs ch
 
-      | C_Wait_Finished2 digestClientFinished, [Finished f], [digestServerFinished] ->
-        client_ServerFinished hs f digestClientFinished
+    | S_Wait_Finished1 digest, [Msg12 (M12_finished f)], [digestClientFinish] ->
+      server_ClientFinished hs f digest digestClientFinish
 
-      | S_Idle, [ClientHello ch], []  -> server_ClientHello hs ch None
-      | S_Idle, [ClientHello ch; Binders binders], []  -> server_ClientHello hs ch (Some binders)
+    | S_Wait_CF2 digest, [Msg12 (M12_finished f)], [digestClientFinished] -> // classic resumption
+      server_ClientFinished2 hs f digest digestClientFinished
 
-      | S_Wait_Finished1 digest, [Finished f], [digestClientFinish] ->
-        server_ClientFinished hs f.fin_vd digest digestClientFinish
-      | S_Wait_Finished1 digest, [Finished f], tags ->
-        trace (TLSConstants.fold_string print_bytes "BAD TAGS: " " " tags);
-        server_ClientFinished hs f.fin_vd digest digest
+    | S_Wait_Finished2 (digestServerFinished),
+      [Msg13 (M13_finished f)], [digestClientFinished] ->
+      server_ClientFinished_13 hs f digestServerFinished digestClientFinished None
 
-      | S_Wait_CF2 digest, [Finished f], [digestClientFinished] -> // classic resumption
-        server_ClientFinished2 hs f.fin_vd digest digestClientFinished
+    | S_Wait_Finished2 (digestServerFinished),
+      [Msg13 (M13_certificate c); Msg13 (M13_certificate_verify cv); Msg13 (M13_finished f)], [digestSigned; digestCertVerify; digestClientFinished] ->
+      server_ClientFinished_13 hs f digestCertVerify digestClientFinished (Some (c, cv, digestSigned))
 
-      | S_Wait_Finished2 (digestServerFinished),
-        [Finished f], [digestClientFinished] ->
-        server_ClientFinished_13 hs f.fin_vd digestServerFinished digestClientFinished None
+    | S_Wait_EOED, [Msg13 (M13_end_of_early_data ())], [digestEOED] ->
+      server_EOED hs digestEOED
 
-      | S_Wait_Finished2 (digestServerFinished),
-        [Certificate13 c; CertificateVerify cv; Finished f], [digestSigned; digestCertVerify; digestClientFinished] ->
-        server_ClientFinished_13 hs f.fin_vd digestCertVerify digestClientFinished (Some (c, cv, digestSigned))
+    | C_Complete, [Msg13 (M13_new_session_ticket st13)], [] ->
+      client_NewSessionTicket_13 hs st13
 
-      | S_Wait_EOED,
-        [EndOfEarlyData], [digestEOED] ->
-        server_EOED hs digestEOED
-
-      | C_Complete, [NewSessionTicket13 st13], [] ->
-        client_NewSessionTicket_13 hs st13
-
-      // are we missing the case with a Certificate but no CertificateVerify?
-      | _,  _, _ ->
-        trace "DISCARD FLIGHT"; InAck false false
-        //InError(AD_unexpected_message, "unexpected flight")
-
-
+    // are we missing the case with a Certificate but no CertificateVerify?
+    | _,  _, _ ->
+      trace "DISCARD FLIGHT"; InAck false false
+      //InError(AD_unexpected_message, "unexpected flight")
 
 // TODO check CCS once committed to TLS 1.3 yields an alert
 let recv_ccs (hs:hs) =
-    trace "recv_ccs";
-    // Draft 22 CCS during HRR
-    // Because of stateless HRR, this may also happen as the very first message before CH (!!!)
-    let is_hrr = Nego.is_hrr hs.nego in
-    let is_idle = S_Idle? !hs.state in
-    if is_hrr || is_idle then
-     begin
-      trace "IGNORING CCS (workaround for implementations that send CCS after HRR)";
-      InAck false false
-     end
-    else
-      // CCS triggers completion of the incoming flight of messages.
-      let mode = Nego.getMode hs.nego in
-      match HandshakeLog.receive_CCS #(Nego.hashAlg mode) hs.log with
-      | Error z -> InError z
-      | Correct (ms, digests, digestCCS) ->
-        match !hs.state, ms, digests with
-        // client resumption
-        | C_Wait_CCS1 _, [NewSessionTicket st], [digestNewSessionTicket] ->
-          client_NewSessionTicket_12 hs true digestNewSessionTicket (Some st)
-        | C_Wait_CCS1 digestServerHello, [], [] ->
-          client_NewSessionTicket_12 hs true digestServerHello None
-        // client full handshake
-        | C_Wait_CCS2 digest, [], [] ->
-          client_NewSessionTicket_12 hs false digest None
-        | C_Wait_CCS2 _, [NewSessionTicket st], [digestNewSessionTicket] ->
-          client_NewSessionTicket_12 hs false digestNewSessionTicket (Some st)
+  let open HandshakeLog in
+  let open HandshakeMessages in
+  trace "recv_ccs";
+  // Draft 22 CCS during HRR
+  // Because of stateless HRR, this may also happen as the very first message before CH (!!!)
+  let is_hrr = Nego.is_hrr hs.nego in
+  let is_idle = S_Idle? !hs.state in
+  if is_hrr || is_idle then
+    begin
+    trace "IGNORING CCS (workaround for implementations that send CCS after HRR)";
+    InAck false false
+    end
+  else
+    // CCS triggers completion of the incoming flight of messages.
+    let mode = Nego.getMode hs.nego in
+    match receive_CCS #(Nego.hashAlg mode) hs.log with
+    | Error z -> InError z
+    | Correct (ms, digests, digestCCS) ->
+      match !hs.state, ms, digests with
+      // client resumption
+      | C_Wait_CCS1 _, [Msg12 (M12_new_session_ticket st)], [digestNewSessionTicket] ->
+        client_NewSessionTicket_12 hs true digestNewSessionTicket (Some st)
+      | C_Wait_CCS1 digestServerHello, [], [] ->
+        client_NewSessionTicket_12 hs true digestServerHello None
+      // client full handshake
+      | C_Wait_CCS2 digest, [], [] ->
+        client_NewSessionTicket_12 hs false digest None
+      | C_Wait_CCS2 _, [Msg12 (M12_new_session_ticket st)], [digestNewSessionTicket] ->
+        client_NewSessionTicket_12 hs false digestNewSessionTicket (Some st)
 
-        | S_Wait_CCS2 digestServerFinished, [], [] -> (
-          Epochs.incr_reader hs.epochs;
-          hs.state := S_Wait_CF2 digestServerFinished;
-          InAck true false)
+      | S_Wait_CCS2 digestServerFinished, [], [] -> (
+        Epochs.incr_reader hs.epochs;
+        hs.state := S_Wait_CF2 digestServerFinished;
+        InAck true false)
 
-        | S_Wait_CCS1, [ClientKeyExchange cke], [digest_to_finish] ->
-          // assert (Some? pv && pv <> Some TLS_1p3 && (kex = Some Kex_DHE || kex = Some Kex_ECDHE))
-          // getting two copies of the same digest?
-          server_ClientCCS1 hs cke digestCCS
+      | S_Wait_CCS1, [Msg12 (M12_client_key_exchange cke)], [digest_to_finish] ->
+        // assert (Some? pv && pv <> Some TLS_1p3 && (kex = Some Kex_DHE || kex = Some Kex_ECDHE))
+        // getting two copies of the same digest?
+        server_ClientCCS1 hs cke digestCCS
 
-        | _, _, _ ->
-          trace "WARNING: bad CCS";
-          InError(fatalAlert Unexpected_message, "CCS received at wrong time")
+      | _, _, _ ->
+        trace "WARNING: bad CCS";
+        InError(fatalAlert Unexpected_message, "CCS received at wrong time")
 
 
 let authorize s ch = FStar.Error.unexpected "authorize: not yet implemented"
